\renewcommand{\theequation}{\theenumi}
\begin{enumerate}[label=\arabic*.,ref=\thesubsection.\theenumi]
\item The equation of a circle is 
\begin{align}
\label{eq:circ_norm}
\norm{\vec{x}-\vec{c}} = r
\end{align}
%
where $\vec{c}$ is the centre and $r$ is the radius.
\item By expanding \eqref{eq:circ_norm}, the equation of a circle can also be expressed as
%
\numberwithin{equation}{enumi}
\begin{align}
\label{eq:circ_quad}
\norm{\vec{x}-\vec{c}}^2 = r^2&
\\
\implies \vec{x}^T\vec{x}-2\vec{c}^T\vec{x} + \vec{c}^T\vec{c}-r^2 = 0
\end{align}
\item Find the equation of a circle that passes through the points $\vec{A},\vec{B},\vec{C}$.
\\
\solution From \eqref{eq:circ_quad},
\begin{align}
%\label{eq:circ_quad}
\norm{\vec{A}-\vec{c}}^2 = \norm{\vec{B}-\vec{c}}^2 = \norm{\vec{C}-\vec{c}}^2 &= r^2
\\
\implies \norm{\vec{A}-\vec{c}}^2 - \norm{\vec{B}-\vec{c}}^2 &=0
\end{align}
which can be simplified to obtain
\begin{align}
\brak{\vec{A}-\vec{B}}^T\vec{c}=\frac{\norm{\vec{A}}^2 - \norm{\vec{B}}^2}{2}& \quad \text{and}
\\
\brak{\vec{A}-\vec{C}}^T\vec{c}=\frac{\norm{\vec{A}}^2 - \norm{\vec{C}}^2}{2}& 
\end{align}
%
Solving the two yields $\vec{c}$, which can then be used to obtain $r$.
\item Let $\vec{A},\vec{B}$ and $\vec{C}$ be three points on the circle and 
$D$ be a point on $BC$ such that
$OD \perp BC$ as in Fig. \ref{fig:ccircle}.  Show that 
\begin{align}
\vec{D}=\frac{\vec{B}+\vec{C}}{2}
\end{align}
%
\begin{figure}[!ht]
	\begin{center}
		
		%\includegraphics[width=\columnwidth]{./figs/ch3_angle_bisector}
		%\vspace*{-10cm}
		\resizebox{\columnwidth}{!}{\input{./figs/ccircle.tex}}
	\end{center}
	\caption{Circumcircle.}
	\label{fig:ccircle}	
\end{figure}


\solution From \eqref{eq:circ_norm}
\begin{align}
\norm{\vec{B}-\vec{O}}^2=\norm{\vec{C}-\vec{O}}^2=r^2
\\
 \implies \brak{\vec{B}-\vec{O}}^T\brak{\vec{B}-\vec{O}} = 
\brak{\vec{C}-\vec{O}}^T\brak{\vec{C}-\vec{O}} 
\\
 \implies \brak{\vec{B}-\vec{C}}^T\brak{\frac{\vec{B}+\vec{C}}{2} - 
\vec{O}}  = 0
\label{eq:circle_mid}
\end{align}
after simplification. Since $OD \perp BC$,
\begin{align}
\brak{\vec{B}-\vec{C}}^T\brak{\vec{D}-\vec{O}} = 0 
\label{eq:circle_D}
\end{align}
Since $D$ and $\frac{\vec{B}+\vec{C}}{2}$ lie on $BC$, using 
\eqref{eq:line_ab},
\begin{align}
\label{eq:circle_mid_D1}
\frac{\vec{B}+\vec{C}}{2}
&= \vec{B}+ \lambda_1\brak{\vec{B}-\vec{C}}
\\
\vec{D}
&= \vec{B}+ \lambda_2\brak{\vec{B}-\vec{C}}
\label{eq:circle_mid_D2}
\end{align}
Multiplying \eqref{eq:circle_mid_D1} and \eqref{eq:circle_mid_D2} with 
$\brak{\vec{B}-\vec{C}}^T$ and subtracting, $\lambda_1=\lambda_2$
%
\begin{align}
\implies \vec{D} = \frac{\vec{B}+\vec{C}}{2}
\label{eq:circle_bisect}
\end{align}
%
\item Let  $\vec{D}$ be the mid point of $BC$.  Show that $OD \perp BC$.
%
\item The circle with centre $\vec{O}$ and radius $r$ in Fig.\ref{fig:ang_bisect}	
 is inside 
$\triangle ABC$ and touches $AB, BC$ 
and $CA$ at $\vec{F}, \vec{D}$ and $\vec{E}$ respectively. $AB, BC$ and 
$CA$ are known as {\em tangents} to the circle.
\begin{figure}[!ht]
	\begin{center}
		
		%\includegraphics[width=\columnwidth]{./figs/ch3_angle_bisector}
		%\vspace*{-10cm}
		\resizebox{\columnwidth}{!}{\input{./figs/ang_bisect.tex}}
	\end{center}
	\caption{Tangent and incircle.}
	\label{fig:ang_bisect}	
\end{figure}


\item Show that $OD \perp BC$.
%\begin{figure}[!h]
%\centering
%\resizebox {\columnwidth} {!} {
%\input{./figs/derivative.tex}
%}
%\caption{Notion of the derivative.}
%\label{fig:derivative}
%\end{figure}
\\
\solution Let $\vec{x}_1,\vec{x}_2$ be two points on the circle such that 
$x_1x_2 \parallel BC$. Then
%
\begin{align}
\norm{\vec{x}_1-\vec{O}}^2- 
\norm{\vec{x}_2-\vec{O}}^2 &= 0 
\\
\implies 
\brak{\vec{x}_1-\vec{x}_2}^T\brak{\frac{\vec{x}_1+\vec{x}_2}{2}-\vec{O}} &= 
0 
\\
\implies 
\brak{\vec{B}-\vec{C}}^T\brak{\frac{\vec{x}_1+\vec{x}_2}{2}-\vec{O}} &= 
0 
%\label{eq:circle_bisect}
\end{align}
%
For $\vec{x}_1=\vec{x}_2=\vec{D}$, $x_1x_2$ merges into $BC$ and the above 
equation becomes 
%
\begin{align}
\brak{\vec{B}-\vec{C}}^T\brak{\vec{D}-\vec{O}} = 
0 
\implies OD \perp BC
%\label{eq:circle_bisect}
\end{align}
%
\item Give an alternative proof for the above.
\\
\solution Let 
\begin{align}
\vec{B} & = \mbf{0}
\\
\vec{D} &= \lambda \vec{m}
\end{align}
Then
\begin{align}
\norm{\vec{D} - \vec{O}}^2 = r^2 &
\\
\implies \lambda^2\norm{\vec{m}}^2 - 2\lambda\vec{m}^T\vec{O} + \norm{\vec{O}}^2 &= r^2 
\end{align}
Since the above equation has a single root,
\begin{align}
\lambda = \frac{\vec{m}^T\vec{O}}{\norm{\vec{m}}^2}
\label{eq:incircle_lam}
\end{align}
%
Thus, 
\begin{align}
\brak{\vec{D} - \vec{B}}^T\brak{\vec{D} - \vec{O}}
&= \brak{\lambda\vec{m}}^T
\brak{\lambda\vec{m}-\vec{O}}
\\
&=\lambda^2\norm{\vec{m}}^2-\lambda\vec{m}^T\vec{O}
\\
&= \mbf{O} \text{ (from \ref{eq:incircle_lam})}.
\\
\implies & OD \perp BC
\end{align}
\item Find the equation of the tangent at $\vec{D}$.
\\
\solution The equation of the tangent is given by 
\begin{align}
\brak{\vec{O}-\vec{D}}^T\brak{\vec{x}-\vec{D}}=0
%\label{eq:circle_bisect}
\end{align}
\end{enumerate}


