\renewcommand{\theequation}{\theenumi}
\begin{enumerate}[label=\arabic*.,ref=\thesubsection.\theenumi]
\numberwithin{equation}{enumi}
%
%
\item Find the distance of the point $\vec{P}=\myvec{3\\-5}$ from the line 
\begin{align}
\label{eq:opt_line_nor}
L: \quad \myvec{3 & – 4}\vec{x}  = 26
\end{align}
\solution Using the equation of the line 
\begin{align}
\label{eq:opt_line_dir}
\vec{x} = \vec{A} + \lambda \vec{m}, 
\end{align}
where $\vec{A}$ is any point on the line and 
\begin{align}
\vec{Q} &= \myvec{0 & -1\\1 & 0}
\\
\vec{n} &= \myvec{3 \\ – 4}
\\
\vec{m} &= \vec{Q}\vec{n} = \myvec{4\\3}
\\
c&=26
\end{align}
%
The distance of $\vec{P}$ from $L$ can be obtained as 
\begin{align}
\min_{\lambda}f(\lambda)
\end{align}
%
where
%
\begin{align}
f(\lambda) &=\norm{\vec{x}-\vec{P}}^2 = \norm{\vec{A} + \lambda \vec{m}-\vec{P}}^2 
\\
& = \brak{ \lambda \vec{m}+\vec{A} -\vec{P}}^T \brak{ \lambda \vec{m}+\vec{A} -\vec{P}}
\\
&= \lambda^2 \norm{\vec{m}}^2 +2\lambda \vec{m}^T\brak{\vec{A} -\vec{P}} 
\nonumber \\
&\quad + \norm{\vec{A} -\vec{P}}^2
\end{align}
\begin{align}
\because f^{(2)}\lambda = 2\norm{\vec{m}}^2 > 0
\end{align}
%
the minimum value of $f(\lambda)$ is obtained when 
%
\begin{align}
\because f^{(1)}\lambda &= 2\lambda\norm{\vec{m}}^2 + 2 \vec{m}^T\brak{\vec{A} -\vec{P}} =0
\\
\implies \lambda_{\min} &= -\frac{\vec{m}^T\brak{\vec{A} -\vec{P}}}{\norm{\vec{m}}^2}
\end{align}
%
Choosing $\vec{A}$ such that 
%
\begin{align}
\vec{m}^T\brak{\vec{A} -\vec{P}} &= 0
\\
\implies \vec{A} -\vec{P} &= \mu \vec{n}
\\
\text{or, } \vec{n}^T	\brak{\vec{A} -\vec{P} } &= \mu \norm{\vec{n}}^2
\\
\implies \mu & = \frac{\vec{n}^T\vec{A} -\vec{n}^T\vec{P} }{\norm{\vec{n}}^2} = \frac{c -\vec{n}^T\vec{P} }{\norm{\vec{n}}^2}
\end{align}
%
where $\mu$ is some constant.
Thus, the shortest distance from $\vec{P}$ to $L$ is
%
\begin{align}
d &= \sqrt{\lambda_{\min}^2 \norm{\vec{m}}^2 +2\lambda_{\min} \vec{m}^T\brak{\vec{A} -\vec{P}
+ \norm{\vec{A} -\vec{P}}^2}}
\\
\implies d &=  \norm{\vec{A} -\vec{P}} = \abs{\mu} \norm{\vec{n}}= \frac{\abs{ \vec{n}^T\vec{P}-c} }{\norm{\vec{n}}}
\end{align}
%
\item Find the equation of the line whose perpendicular distance from the origin is 4 units and the angle which the normal makes with the positive direction of x-axis is $15\degree$.
\\
\solution 
%
\item Find the 
distance between the lines 
\begin{align}
L_1: \quad \vec{x} &= \myvec{1\\2\\-4} + \lambda_1\myvec{2 \\ 3 \\6}
\\
L_2: \quad \vec{x} &= \myvec{3\\3\\-5} + \lambda_2\myvec{2 \\ 3 \\6}
\end{align}
\label{prob:line_dist_parallel}
%


\item Find the shortest distance between the lines 
\begin{align}
L_1: \quad \vec{x} &= \myvec{1\\1\\0} + \lambda_1\myvec{2 \\ -1 \\1}
\\
L_2: \quad \vec{x} &= \myvec{2\\1\\-1} + \lambda_2\myvec{3 \\ -5 \\2}
\end{align}
\label{prob:line_dist_skew}
%


\item Find the distance of the plane 
\begin{align}
\myvec{2 & -3 & 4}\vec{x}-6  = 0
\end{align}
%
from the origin.


\item Find the equation of a plane which is at a distance of $\frac{6}{\sqrt{29}}$ from the origin and has  normal vector $\vec{n}=\myvec{2\\-3\\4}$.
%
\\
\solution From the previous problem, the desired equation is
%
\begin{align}
\myvec{2 & -3 & 4}\vec{x}-6  = 0
\end{align}
%

\item Find the unit normal vector of the plane 
\begin{align}
\myvec{6 & -3 & -2}\vec{x}  = 1.
\end{align}
%
\solution The normal vector is 
%
\begin{align}
\vec{n} = \myvec{6 & -3 & -2}
\\
\because \norm{\vec{n}} = 7,
\end{align}
%
the unit normal vector is 
%
\begin{align}
\frac{\vec{n}}{\norm{\vec{n}}} = \frac{1}{7}\myvec{6 & -3 & -2}
\end{align}
%
\item Find the coordinates of the foot of the perpendicular drawn from the origin to the plane 
\begin{align}
\label{eq:line_foot_perp}
\myvec{2 & -3 & 4}\vec{x}-6  = 0
\end{align}
%
\solution The normal vector is 
%
\begin{align}
\vec{n}=\myvec{2 \\ -3 \\ 4}
\end{align}
%
Hence, the foot of the perpendicular from the origin is $\lambda \vec{n}$.  Substituting in \eqref{eq:line_foot_perp},
\begin{align}
\lambda \norm{\vec{n}}^2 = 6  \implies \lambda = \frac{6}{\norm{\vec{n}}^2} = \frac{6}{29}
\end{align}
%
Thus, the foot of the perpendicular is
%
\begin{align}
\frac{6}{29}\myvec{2 \\ -3 \\ 4}
\end{align}
%
\item Find the equation of the plane which passes through the point $\vec{A}=\myvec{5\\2\\-4}$ and perpendicular to the line with direction vector $\vec{n}=\myvec{2\\3\\-1}$.
%
\\
\solution  The normal vector to the plane is $\vec{n}$. Hence from \eqref{eq:line_norm_vec}, the equation of the plane is 
%
\begin{align}
\vec{n}^T\brak{\vec{x}-\vec{A}} &= 0
\\
\implies \myvec{2\\3\\-1}\vec{x} &=\myvec{2&3&-1}\myvec{5\\2\\-4}
\\
&=20
\end{align}
%
%The following 
%%
%\begin{lstlisting}
%codes/line/plane_3d.py
%\end{lstlisting}
%%
%\begin{figure}[!ht]
%\includegraphics[width=\columnwidth]{./line/figs/plane_3d.eps}
%\caption{}
%\label{fig:plane_3d}
%\end{figure}
%

\item Find the equation of the plane passing through 
$
\bm{R} = \myvec{2\\5\\-3},
\bm{S}= \myvec{-2\\-3\\5}
$ 
and 
$
\bm{T}= \myvec{5\\3\\-3}.
$
\label{prob:plane_3pts}
\\
\solution  If the equation of the plane be 
\begin{align}
\vec{n}^T\vec{x} &= c,
\\
\vec{n}^T\vec{R}=\vec{n}^T\vec{S}=\vec{n}^T\vec{T}&= c,
\\
\implies \myvec{\vec{R}-\vec{S} & \vec{S}-\vec{T}}^T\vec{n} &= 0
\end{align}
%
after some algebra.
Using row reduction on the above matrix, 
\begin{align}
\myvec{4 & 8 &-8 \\ -7  & -6 & 8} \xleftrightarrow[]{R_1\leftarrow \frac{R_1}{4}}\myvec{1 & 2 &-2 \\ -7  & -6 & 8}
\\
\xleftrightarrow[]{R_2\leftarrow R_2 + 7R_1}
\myvec{
1 & 2 &-2 
\\ 
0  & 8 & -6
}
\xleftrightarrow[]{R_2\leftarrow \frac{R_2}{2}}
\myvec{
1 & 2 &-2 
\\ 
0  & 4 & -3
}
\\
\xleftrightarrow[]{R_1\leftarrow 2R_1-R_2}
\myvec{
2 & 0 &-1 
\\ 
0  & 4 & -3
}
\end{align}
%
Thus, 
\begin{align}
\vec{n} &= \myvec{\frac{1}{2}\\\frac{3}{4}\\1} = \myvec{2\\3\\4} \text{ and}
\\
c = \vec{n}^{T}\vec{T} = 7
\end{align}
%
Thus, the equation of the plane is 
%
\begin{align}
\myvec{2 & 3 & 4}\vec{n} = 7
\end{align}
%
Alternatively, the normal vector to the plane can be obtained as
%
\begin{align}
\vec{n} = \brak{\vec{R}-\vec{S}} \times \brak{\vec{S}-\vec{T}}
\end{align}
%
The equation of the plane is then obtained from \eqref{eq:line_norm_vec} as 
%
\begin{align}
\label{eq:plane_3pts_cross}
\vec{n}^T\brak{\vec{x}-\vec{T}} = \sbrak{\brak{\vec{R}-\vec{S}} \times \brak{\vec{S}-\vec{T}}}^T\brak{\vec{x}-\vec{T}} = 0
\end{align}
%

\item Find the equation of the plane with intercepts 2, 3 and 4 on the x, y and z axis respectively.
\\
\solution From the given information, the plane passes through the points \myvec{2\\0\\0}, \myvec{0\\3\\0} and \myvec{0\\0\\4} respectively. The equation can be obtained using Problem \ref{prob:plane_3pts}.

\item Find the equation of the plane passing through the intersection of the planes 
%
\begin{align}
\label{eq:plane_2p_1pt_1}
\myvec{1 & 1 & 1}\vec{x}&=6  
\\
\myvec{2 & 3 & 4}\vec{x}&=-5
\label{eq:plane_2p_1pt_2}
\end{align}
%
and the point \myvec{1\\1\\1}.
\\
\solution The intersection of the planes is obtained by row reducing the augmented matrix as
%
\begin{align}
\myvec{
1 & 1 & 1 & 6
\\
2 & 3 & 4 & -5
}
\xleftrightarrow[]{R_2 = R_2 -2R_1}
\myvec{
1 & 1 & 1 & 6
\\
0 & 1 & 2 & -17
}
\\
\xleftrightarrow[]{R_1 = R_1 -R_2}
\myvec{
1 & 0 & -1 & 23
\\
0 & 1 & 2 & -17
}
\\
\implies 
\vec{x} = \myvec{23\\-17\\0}+\lambda\myvec{1\\-2\\1}
\end{align}
%
Thus, \myvec{23\\-17\\0} is another point on the plane.  The normal vector to the plane is then obtained as
The normal vector to the plane is then obtained as
%
\begin{align}
\brak{ \myvec{1\\1\\1}-\myvec{23\\-17\\0}}\times \myvec{1\\-2\\1} 
\end{align}
%
which can be obtained by row reducing the matrix
\begin{align}
\myvec{
1 & -2 & 1
\\
-22 & 18 & 1
}
\xleftrightarrow[]{R_2 = R_2+22R_1}
\myvec{
1 & -2 & 1
\\
0  & -26 & 23
}
\\
\xleftrightarrow[]{R_1 = 13R_1-R_2}
\myvec{
13 & 0 & -10
\\
0  & -26 & 23
}
\\
\implies \vec{n} = \myvec{\frac{10}{13}\\\frac{23}{26}\\1} = \myvec{20\\23\\26}
\end{align}
%
Since the plane passes through \myvec{1\\1\\1}, using 
 \eqref{eq:line_norm_vec},
%
\begin{align}
\myvec{20 & 23 & 26}\brak{\vec{x}- \myvec{1\\1\\1}} &= 0
\\
\implies 
\myvec{20 & 23 & 26}\vec{x} &= 69
\end{align}
%
Alternatively, the plane passing through the intersection of \eqref{eq:plane_2p_1pt_1} and 
\eqref{eq:plane_2p_1pt_2} has the form 
%
\begin{align}
\label{eq:plane_2p_1pt_lam}
\myvec{1 & 1 & 1}\vec{x} + \lambda \myvec{2 & 3 & 4}\vec{x} &=6 -5\lambda  
\end{align}
%
Substituting \myvec{1\\1\\1} in the above, 
%
\begin{align}
\myvec{1 & 1 & 1}\myvec{1\\1\\1} + \lambda \myvec{2 & 3 & 4}\myvec{1\\1\\1} &=6 -5\lambda  
\\
\implies 3 + 9\lambda &= 6-5\lambda
\\
\implies &\lambda = \frac{3}{14}
\end{align}
%
Substituting this value of $\lambda $ in \eqref{eq:plane_2p_1pt_lam} yields the equation of the plane.

\item Show that the lines 
\label{prob:line_coplanar}
%
\begin{align}
\frac{x+3}{-3} = \frac{y-1}{1} &= \frac{z-5}{5}, 
\\
\frac{x+1}{-1} = \frac{y-2}{2} &= \frac{z-5}{5} 
\end{align}
%
are coplanar.

\item Find the distance of a point \myvec{2\\5\\-3} from the plane
\begin{align}
\myvec{6 & -3 & 2}\vec{x}=4
\end{align}
%

\item Find the distance between the point $\vec{P}=\myvec{6\\5\\9}$ and the plane determined by the points $\bm{A}=\myvec{3\\-1\\2}, \bm{B}=\myvec{5\\2\\4}$ and $\bm{C}=\myvec{-1\\-1\\6}$.
%
%
\end{enumerate}
