\begin{enumerate}[1.]
\item What does the equation 
\begin{align*}
x^2-y^2-4x-6y-6=0
\end{align*}
become when the origin is moved to the point $\brak{2,-3}$?
\item To what point must the origin be moved in order that the equation
\begin{align*}
2x^2-3xy+4y^2+10x - 19y + 23 = 0
\end{align*}
may become
\begin{align*}
2x^2-3xy+4y^2 = 1
\end{align*}
\item Show that the equation
\begin{align*}
x^2+y^2 = a^2
\end{align*}
remains unaltered by any rotation of the axes.
\item What does the equation
\begin{align*}
x^2+2\sqrt{3}xy - y^2 = 2a^2
\end{align*}
become when the axes are turned through $30\degree$?
\item What does the equation
\begin{align*}
\brak{y-x}^2 = 4\sqrt{2}a\brak{x+y}
\end{align*}
become when the axes are turned through $45\degree$?
\item To what point must the origin be moved in order that the equation
\begin{align*}
x^2+4xy-2y^2+10x-4y = 0
\end{align*}
may become
\begin{align*}
x^2+4xy-2y^2 = 1
\end{align*}
and through what angle must the axes be turned in order to get rid
of the term in $xy$?
\item Through what angle must the axes be turned to reduce the equation
\begin{align*}
x^2-2xy-y^2 = 1
\end{align*}
to the form
\begin{align*}
xy = c
\end{align*}
where $c$ is a constant.
\item Show that, by changing the origin, the equation
\begin{align*}
2x^2+2y^2+7x+5y-13 = 0
\end{align*}
can be transformed to 
\begin{align*}
8x^2+8y^2 = 89
\end{align*}
\item Show that, by rotating the axes, the equation
\begin{align*}
3x^2+7xy-3y^2 = 1
\end{align*}
can be reduced to 
\begin{align*}
\sqrt{85}\brak{x^2-y^2}=2
\end{align*}
\item Show that, by rotating the axes, the equation
\begin{align*}
41x^2+24xy+34y^2=75
\end{align*}
can be reduced to 
\begin{align*}
2x^2+y^2 = 3
\end{align*}
\item Show that, by a change of origin and the directions of the coordinate axes, the equation
\begin{align*}
5x^2+2xy+5y^2-14x-22y+27=0
\end{align*}
can be transformed to
\begin{align*}
3x^2+2y^2 = 1
\end{align*}
or
\begin{align*}
2x^2+3y^2 = 1
\end{align*}
\end{enumerate}