\subsection{Definitions}

\begin{definition}
{\em (Circle):} Fig. \ref{fig:ch3_circle_def} shows a circle with centre $O$ and radius $r$, where each point on the circle is at the same distance $r$ from the centre $O$.
\end{definition}
%%
\begin{figure}[!h]
\centering
\resizebox {\columnwidth} {!} {
\input{./figs/chapter3/ch3_circle_def.tex}
}
\caption{Circle with radius $r$.}
\label{fig:ch3_circle_def}
\end{figure}
%
\begin{problem}
Show that the equation of the circle is 
%
\begin{equation}
\label{eq:ch3_circle_def}
\brak{x-a}^2 + \brak{y-b}^2 = r^2
\end{equation}
%
\end{problem}
\proof Since each point $\brak{x,y}$ on the circle is at a distance $r$ from the centre $\brak{a,b}$, using \eqref{eq:ch1_distance}, \eqref{eq:ch3_circle_def} is obtained.
%
\begin{definition}
{\em (Tangent)}: In Fig. \ref{fig:ch3_tangent_def},  the line $BX$ that touches the circle at exactly one point $C$ is known as the tangent.
\end{definition}
%
\begin{figure}[!h]
\centering
\resizebox {\columnwidth} {!} {
\input{./figs/chapter3/ch3_tangent_def.tex}
}
\caption{Tangent to the circle.}
\label{fig:ch3_tangent_def}
\end{figure}
%
\subsection{Tangent}
\begin{problem}
In Fig. \ref{fig:ch3_tangent_def}, show that the tangent $BX \perp OC$. 
\end{problem}
\proof Since $C$ lies on the circle and is at distance $r$ from the centre $O$, using \eqref{eq:ch1_distance},
%
\begin{align}
\brak{x-a}^2 + b^2 &= r^2
\\
\Rightarrow x = a \pm \sqrt{r^2-b^2}
\label{eq:ch3_c_two_sol}
\end{align}
%
By the definition of a tangent, the point $C$ should be unique.  Thus, in \eqref{eq:ch3_c_two_sol}, $x = a$ and $r = b$. By definition of the coordnate system, this implies that $\Delta OCB$ is right angled and $BX \perp OC$.
\begin{problem}
In Fig. \ref{fig:ch3_tangent_intercept}, $BX$ is a tangent to the circle centred at $O$ and touches it at $C$.  $P$ and $Q$ are two points on the circle.  Show that
\begin{equation}
\label{eq:ch3_tangent_intercept}
BP.BQ = BC^2
\end{equation}
\end{problem}
%
\begin{figure}[!h]
\centering
\resizebox {\columnwidth} {!} {
\input{./figs/chapter3/ch3_tangent_intercept.tex}
}
\caption{$BP.BQ = BC^2$.}
\label{fig:ch3_tangent_intercept}
\end{figure}
%

\proof Let $m$ be the slope of the line $BQ$.  Then the coordinates of $P$ and $Q$ can be represented as $\brak{p,mp}$ and $\brak{q,mq}$ respectively. The radius of the circle is $b$.  Using \eqref{eq:ch3_circle_def} for $P$ and $Q$, 
%
\begin{align}
\brak{p-a}^2 + \brak{mp-b}^2 &= b^2
\\
\Rightarrow a^2 -2ap + m^2p^2 &= 2mpb
\label{eq:ch3_p_circ}
\end{align}
and
\begin{align}
\Rightarrow a^2 -2aq + m^2q^2 &= 2mqb
\label{eq:ch3_q_circ}
\end{align}
%
Dividing \eqref{eq:ch3_p_circ} by \eqref{eq:ch3_q_circ},
\begin{align}
\frac{a^2 -2ap + p^2\brak{1+m^2}}{a^2 -2aq + q^2\brak{1+m^2}} &= \frac{p}{q}
\end{align}
which, after cross multiplying, results in
\begin{multline}
q\brak{a^2 -2ap + p^2\brak{1+m^2}} 
\\
= p \brak{a^2 -2aq + q^2\brak{1+m^2}}
\end{multline}
and can be simplified as
\begin{align}
a^2\brak{p-q}  &= pq\brak{p-q}\brak{1+m^2} 
\\
\Rightarrow
a^2  &= pq\brak{1+m^2} 
\\
\Rightarrow a^2 &=  p\sqrt{\brak{1+m^2}}.q\sqrt{\brak{1+m^2}}
\\
\Rightarrow BC^2 &= BP.BQ,
\end{align}
using \eqref{eq:ch1_distance} for obtaining the length of $BP$ and $BQ$.
\subsection{Semi-circle}
%
\begin{problem}
Fig. \ref{fig:ch3_semi_circle} shows a semi circle.  $BC = 2r$, where $r$ is the radius of the circle is known as the diameter.  Show that $\angle BAC = 90^{\degree}$.
\end{problem}
\begin{figure}[!h]
\centering
\resizebox {\columnwidth} {!} {
\input{./figs/chapter3/ch3_semi_circle.tex}
}
\caption{$\angle BAC = 90^{\degree}$.}
\label{fig:ch3_semi_circle}
\end{figure}
%
\proof From \eqref{eq:ch3_circle_def},
\begin{align}
\label{eq:ch3_semi_circle_1}
\brak{a-r}^2 + b^2 &= r^2.
\end{align}
%
From \eqref{eq:ch1_distance},
%
\begin{align}
AB^2 + BC^2 &= \brak{a^2 +b^2} + \brak{a-2r}^2 + b^2
\\
& = 2\brak{a^2 - 2ar +b^2 + r^2} + 2r^2
\\
& = 2\sbrak{\brak{a-r}^2 +b^2} + 2r^2
\\
& = 4r^2 \quad \brak{\text{from \eqref{eq:ch3_semi_circle_1} }}
\\
&= BC^2
\end{align}
From Budhayana's thorem, $\angle ABC = 90^{\degree}$. 
\subsection{More Properties}
\begin{problem}
In Fig. \ref{fig:angle_arc}, show that 
\begin{equation}
\angle BOC = 2 \angle BAC
\end{equation}
\end{problem}
\begin{figure}[!h]
\centering
\resizebox {\columnwidth} {!} {
%\includegraphics[width=\columnwidth]{./figs/chapter3/angle_arc.eps}
\input{./figs/chapter3/angle_arc.tex}
}
\caption{$\theta_1= 2 \theta_2.$}
\label{fig:angle_arc}
\end{figure}
%
\solution In Fig. \ref{fig:angle_arc}, $O$ lies on the $y$-axis.  Hence, t	he radius of the circle is $r$. Since $C$ is a point on the circle,
using the equation of the circle,
\begin{align}
x_1^2+\brak{m_1x-r}^2 = r^2
\\
\Rightarrow x_1\brak{1+m_1^2} = 2m_1 r
\\
\Rightarrow r = \frac{x_1\brak{1+m_1^2}}{2m_1}
\end{align}
%
Since a similar property holds for the point $B$, 
\begin{equation}
\label{eq:rx1x2}
\Rightarrow r = \frac{x_1\brak{1+m_1^2}}{2m_1} = \frac{x_2\brak{1+m_2^2}}{2m_2} 
\end{equation}
From \eqref{eq:ch1_line_ang},
\begin{align}
\tan\theta_1 &= \frac{\frac{m_1x_1-r}{x_1}- \frac{m_2x_2-r}{x_2}}{1+\frac{m_1x_1-r}{x_1}\frac{m_2x_2-r}{x_2}}
\\
&= \frac{m_1-\frac{r}{x_1}- \brak{m_2 - \frac{r}{x_2}}}{1+\brak{m_1-\frac{r}{x_1}}\brak{m_2-\frac{r}{x_2}}}
\end{align}
From \eqref{eq:rx1x2},
\begin{align}
m_1-\frac{r}{x_1} &= \frac{m_1^2-1}{2m_1}
\\
m_2-\frac{r}{x_2} &= \frac{m_2^2-1}{2m_2}
\end{align}
Hence,
\begin{align}
\tan\theta_1 &=  \frac{\frac{m_1^2-1}{2m_1}-\frac{m_2^2-1}{2m_2}}{1+\frac{m_1^2-1}{2m_1}\cdot\frac{m_2^2-1}{2m_2}}
\\
&= \frac{2\brak{m_1-m_2}\brak{1+m_1m_2}}{\brak{4m_1m_2}+\brak{m_1^2-1}\brak{m_2^2-1}}
\end{align}
Again, using \eqref{eq:ch1_line_ang} for $\theta_2$,
\begin{align}
\tan \theta_2 &= \frac{m_1-m_2}{1+m_1m_2}
\\
\Rightarrow \tan2\theta_2 &= \frac{2\tan\theta_2}{1-\tan^2\theta_2} 
\\
&= \frac{2\frac{m_1-m_2}{1+m_1m_2}}{1-\brak{\frac{m_1-m_2}{1+m_1m_2}}^2}
\\
&= \frac{2\brak{m_1-m_2}\brak{1+m_1m_2}}{\brak{1+m_1m_2}^2-\brak{m_1-m_2}^2}
\\
&= \tan\theta_1
\end{align}
after simplification. \qed
\begin{problem}
In Fig. \ref{fig:angle_chord}, show that
\begin{equation}
\angle PBC = \angle BAC.
\end{equation}
\end{problem}
\begin{figure}[!h]
\centering
\resizebox {\columnwidth} {!} {
%\includegraphics[width=\columnwidth]{./figs/chapter3/angle_arc.eps}
\input{./figs/chapter3/angle_chord.tex}
}
\caption{$\theta_1=\theta_2$}
\label{fig:angle_chord}
\end{figure}
\solution
The slopes of $AB, BC, CA$ are, respectively,
\begin{align}
m_{AB} &= m_1 
\\
m_{BC} &= m_2 =\tan\theta_1
\\
m_{CA} &= \frac{m_2x_2-m_1x_1}{m_2-m_1}
\end{align}
From \eqref{eq:ch1_line_ang},
\begin{align}
\tan \theta_2 &= \frac{\frac{m_2x_2-m_1x_1}{m_2-m_1}-m_1}{1+m_1\cdot\frac{m_2x_2-m_1x_1}{m_2-m_1}} 
\\
&= \frac{x_2\brak{m_2-m_1}}{x_2\brak{1+m_1m_2}-x_1\brak{1+m_1^2}}
\\
&= \frac{\brak{m_2-m_1}}{\brak{1+m_1m_2}-\frac{x_1}{x_2}\brak{1+m_1^2}}
\label{eq:angle_chord_theta_2}
\end{align} 
after simplification. From \eqref{eq:rx1x2},
\begin{equation}
\label{eq:x1byx2}
\frac{x_1}{x_2} = \frac{m_1}{m_2}\cdot\frac{\brak{1+m_2^2}}{\brak{1+m_1^2}} 
\end{equation}
%
Substituting \eqref{eq:x1byx2} in \eqref{eq:angle_chord_theta_2},
\begin{align}
\tan \theta_2 &= \frac{\brak{m_2-m_1}}{\brak{1+m_1m_2}-\frac{m_1}{m_2}\cdot\frac{\brak{1+m_2^2}}{\brak{1+m_1^2}} \brak{1+m_1^2}}
\\
&= \frac{\brak{m_2-m_1}}{\brak{1+m_1m_2}-\frac{m_1}{m_2}{\brak{1+m_2^2}}}
\\
&= m_2 = \tan\theta_1 
\end{align}
after simplification \qed.